monadproofs/proofs/evmmisc.v
@@ -1,0 +1,84 @@
+Require Import monad.proofs.bigauto.
+Require Import monad.proofs.evmopsem.
+Require Import monad.proofs.misc.
+Require Import bluerock.hw_models.utils.
+Require Import bluerock.auto.cpp.tactics4.
+
+#[only(lens)] derive block.block_account.
+#[only(lens)] derive AccountM.
+
+(* move to evmmisc.v *)
+
+Definition zbvfun (fz: Z -> Z) (w: keccak.w256): keccak.w256:=
+  let wnz := fz (w256_to_Z w) in
+  Z_to_w256 wnz.
+
+Definition nbvfun (fz: N -> N) (w: keccak.w256): keccak.w256:=
+  let wnz := fz (w256_to_N w) in
+  Z_to_w256 (Z.of_N wnz).
+
+
+Definition zbvlens {A:Type} (l: Lens A A keccak.w256 keccak.w256): Lens A A Z Z :=
+  {| view := λ a : A, w256_to_Z (a .^ l);
+    Lens.over := λ (fz : Z → Z) (a : A), (l %= zbvfun fz) a |}.
+
+Definition nbvlens {A:Type} (l: Lens A A keccak.w256 keccak.w256): Lens A A N N :=
+  {| view := λ a : A, w256_to_N (a .^ l);
+    Lens.over := λ (fz : N → N) (a : A), (l %= nbvfun fz) a |}.
+
+
+Definition _balance : Lens AccountM AccountM Z Z:=
+  zbvlens (_coreAc .@ _block_account_balance).
+
+Definition _balanceN : Lens AccountM AccountM N N :=
+  nbvlens (_coreAc .@ _block_account_balance).
+
+#[global] Instance inh : Inhabited AccountM := populate dummyAc.
+Definition updateBalanceOfAc (s: evm.GlobalState) (addr: evm.address) (upd: N -> N) : evm.GlobalState :=
+  <[ addr :=  (s !!! addr) &: _balanceN %= upd ]> s.
+
+
+Lemma balanceOfUpd s ac f acp:
+  balanceOfAc (updateBalanceOfAc s ac f) acp = if (bool_decide (ac=acp)) then f (balanceOfAc s ac) else (balanceOfAc s acp).
+Proof.
+  simpl.
+  unfold updateBalanceOfAc.
+  unfold balanceOfAc.
+  autorewrite with syntactic.
+  rewrite lookup_insert_iff;[| exact dummyAc].
+  case_bool_decide;  auto.
+  unfold lookup_total.
+  unfold fin_maps.map_lookup_total.
+  unfold default.
+  unfold evm.account_state.
+  case_match; auto.
+  2:{
+    setoid_rewrite H0.
+    unfold inhabitant.
+    simpl.
+    unfold nbvfun.
+    admit.
+  }
+  {
+    setoid_rewrite H0.
+    destruct a.
+    destruct coreAc.
+    simpl.
+    unfold nbvfun.
+    admit.
+  }
+Admitted.
+
+
+
+Ltac resdec tac :=
+  repeat match goal with
+  | [|- context [decide ?P] ] =>
+    resultsIn0or1Goals ltac:(destruct (decide P); try solve [ tac ])
+  | [|- context [bool_decide ?P] ] =>
+    resultsIn0or1Goals ltac:(rewrite (bool_decide_decide P); (destruct (decide P); try solve [ tac ]))
+  | [H:context [decide ?P] |- _ ] =>
+    resultsIn0or1Goals ltac:((destruct (decide P); try solve [ tac ]))
+  | [H:context [bool_decide ?P] |- _ ] =>
+    resultsIn0or1Goals ltac:(rewrite (bool_decide_decide P) in H; (destruct (decide P); try solve [ tac ]))
+    end.
